Realize well-foundedness axioms in BV_Gen.v

lib/coq/WellFounded.v
@@ -1,7 +1,7 @@
 (********************************************************************)
 (*                                                                  *)
 (*  The Why3 Verification Platform   /   The Why3 Development Team  *)
-(*  Copyright 2010-2022 --  Inria - CNRS - Paris-Saclay University  *)
+(*  Copyright 2010-2023 --  Inria - CNRS - Paris-Saclay University  *)
 (*                                                                  *)
 (*  This software is distributed under the terms of the GNU Lesser  *)
 (*  General Public License version 2.1, with the special exception  *)
@@ -11,16 +11,8 @@
 
 Require Import BuiltIn.
 
-Definition func : forall (a:Type) (b:Type), Type.
-Proof.
-intros a b.
-exact (a -> b).
-Defined.
+Definition acc {a:Type} (r:a -> a -> bool) : a -> Prop :=
+  Acc (fun y x => r y x = true).
 
-Definition infix_at: forall {a:Type} {b:Type}, (a -> b) -> a -> b.
-Proof.
-intros a b f x.
-exact (f x).
-Defined.
-
-Definition pred (a: Type) := a -> bool.
+Definition well_founded {a:Type} (r:a -> a -> bool) : Prop :=
+  well_founded (fun y x => r y x = true).
